Tried to modularize Paxos.thy using locales. Not sure it's very useful...

Isabelle2/Paxos.thy
@@ -2,353 +2,36 @@ theory Paxos
 imports "/home/nano/Documents/IO-Automata/IOA_Automation"  "~~/src/HOL/Eisbach/Eisbach_Tools"
   "/home/nano/Documents/IO-Automata/Simulations" "~~/src/HOL/Library/Monad_Syntax"
   "~~/src/HOL/Library/FSet"
-  LinorderOption
+   Quorums BallotArrays
 begin
 
-section {* State and actions of the Paxos algorithm *}
+section {* paxos IOA *}
 
-datatype ('v,'acc,'l) p_action =
+subsection {* State and actions of the paxos algorithm *}
+
+datatype ('v,'a,'l) p_action =
   Propose 'v
 | Learn 'v 'l
-| Vote 'acc
-| JoinBallot nat 'acc
+| Vote 'a
+| JoinBallot nat 'a
 | StartBallot nat
 
-(* Note: using 'b::linorder confuses the record package. *)
-record ('v, 'acc, 'b) p_state =
+record ('v, 'a) p_state =
   propCmd :: "'v fset"
-  ballot :: "'acc \<Rightarrow> 'b option"
-  vote :: "'acc \<Rightarrow> 'b \<Rightarrow> 'v option"
-  suggestion :: "'b \<Rightarrow> 'v option"
+  ballot :: "'a \<Rightarrow> nat option"
+  vote :: "'a \<Rightarrow> nat \<Rightarrow> 'v option"
+  suggestion :: "nat \<Rightarrow> 'v option"
     -- {* The suggestion of the leader of round b *}
 
-section {* Properties of the state *}
+print_locale ballot_array
 
-locale Paxos = IOA +
-  fixes acceptors::"'acc fset" and learners::"'l fset" and quorums::"'acc fset fset"
-  assumes "acceptors \<noteq> {||}"
-    and "learners \<noteq> {||}"
-    and "\<And> q1 q2 . \<lbrakk>q1 |\<in>| quorums; q2 |\<in>| quorums\<rbrakk> \<Longrightarrow> q1 |\<inter>| q2 \<noteq> {||}"
-    and "\<And> q . q |\<in>| quorums \<Longrightarrow> q |\<subseteq>| acceptors"
-    and "quorums \<noteq> {||}"
+locale paxos = IOA + quorums +
+  fixes learners::"'l fset" 
+  assumes "learners \<noteq> {||}"
 begin
 
 text {* If Nitpick can find a model then the assumptions are not contradictory *}
 lemma False nitpick oops
-
-text {* A state is conservative when for every ballot b: if a1 and a2 have voted in b, 
-  then their vote is the same *}
-
-definition conservative where
-  "conservative r b \<equiv> \<forall> a1 . \<forall> a2 . a1 |\<in>| acceptors \<and> a2 |\<in>| acceptors \<longrightarrow> (
-    let v1 = (vote r) a1 b; v2 = (vote r) a2 b in 
-      (v1 \<noteq> None \<and> v2 \<noteq> None) \<longrightarrow> v1 = v2)"
-
-definition conservative_array where
-  "conservative_array r \<equiv> \<forall> b . conservative r b"
-
-text {* Here the max is the one from Lattices_Big *}
-
-definition max_voted_round where
-  "max_voted_round r a bound \<equiv> Max {b . vote r a b \<noteq> None \<and> b \<le> bound}"
-  
-definition max_voted_round_q where
-  "max_voted_round_q r q bound \<equiv> 
-    if \<exists> b a . a |\<in>| q \<and> b \<le> bound \<and> vote r a b \<noteq> None
-    then Some (Max {b . \<exists> a . a |\<in>| q \<and> b \<le> bound \<and> vote r a b \<noteq> None})
-    else None"
-
-lemma finite_voted_bals:"finite {b::nat . \<exists> a . a |\<in>| q \<and> b \<le> bound \<and> vote r a b \<noteq> None}"
-proof -
-  have "{b . \<exists> a . a |\<in>| q \<and> b \<le> bound \<and> vote r a b \<noteq> None} \<subseteq> {b . b \<le> bound}"
-    by auto
-  moreover have "finite {b::nat . b \<le> bound}" by simp
-  ultimately show ?thesis
-  by (metis (no_types, lifting) finite_subset) 
-qed
-
-lemma max_voted_round_none:
-  assumes "a |\<in>| q" and "(b::nat) \<le> bound" 
-  and "max_voted_round_q r q bound = None \<or> b > the (max_voted_round_q r q bound)"
-  shows "vote r a b = None"
-proof (cases "max_voted_round_q r q bound")
-case None 
-  thus ?thesis using assms(1,2)
-  by (auto simp add:max_voted_round_q_def split:split_if_asm)
-next
-  case (Some b\<^sub>m\<^sub>a\<^sub>x)
-  with this obtain a2 b2 v where "a2 |\<in>| q \<and> b2 \<le> bound \<and> vote r a2 b2 = Some v"
-  by (auto simp add:max_voted_round_q_def split:split_if_asm)
-  hence "{b . \<exists> a . a |\<in>| q \<and> b \<le> bound \<and> vote r a b \<noteq> None} \<noteq> {}" by auto
-  with this obtain b2 a2 where "a2 |\<in>| q \<and> b2 \<le> bound \<and> vote r a2 b2 \<noteq> None"
-    by auto
-  moreover note finite_voted_bals
-  moreover have "b > Max {b . \<exists> a . a |\<in>| q \<and> b \<le> bound \<and> vote r a b \<noteq> None}" using Some assms(3)
-    by (auto simp add:max_voted_round_q_def split:split_if_asm)
-  ultimately
-  show ?thesis by (metis (mono_tags, lifting) Max.coboundedI assms(1,2) leD mem_Collect_eq) 
-qed
-
-lemma max_voted_round_some :
-  assumes "max_voted_round_q r q (bound::nat) = Some (b::nat)"
-  obtains a where "a |\<in>| q" and "vote r a b \<noteq> None" and "b \<le> bound"
-proof -
-  from assms have "b = Max {b . \<exists> a . a |\<in>| q \<and> b \<le> bound \<and> vote r a b \<noteq> None}"
-    by (auto simp add:max_voted_round_q_def split:split_if_asm)
-  moreover note finite_voted_bals
-  moreover obtain a2 b2 where "a2 |\<in>| q \<and> b2 \<le> bound \<and> vote r a2 b2 \<noteq> None"
-    using assms by (auto simp add:max_voted_round_q_def) (metis option.distinct(1))
-  ultimately show ?thesis using that
-  by (smt Max_in empty_iff finite_nat_set_iff_bounded_le mem_Collect_eq) 
-qed
- 
-definition max_vote where
-  "max_vote r q bound \<equiv>
-    case max_voted_round_q r q bound of
-      None \<Rightarrow> None
-    | Some b \<Rightarrow> 
-        let max_voter = (SOME a . a |\<in>| q \<and> vote r a b \<noteq> None)
-        in (vote r) max_voter b"
-
-lemma max_vote_some_prop:
-  assumes "max_vote r q (bound::nat) = Some v"
-  obtains a b\<^sub>m\<^sub>a\<^sub>x where "vote r a b\<^sub>m\<^sub>a\<^sub>x = max_vote r q bound" and "a |\<in>| q"
-  and "\<And> a2 b2 . \<lbrakk>a2 |\<in>| q; b2 > b\<^sub>m\<^sub>a\<^sub>x; b2 \<le> bound\<rbrakk> \<Longrightarrow> vote r a2 b2 = None"
-  and "b\<^sub>m\<^sub>a\<^sub>x \<le> bound"
-proof -
-  from assms obtain b\<^sub>m\<^sub>a\<^sub>x where 0:"max_voted_round_q r q bound = Some (b\<^sub>m\<^sub>a\<^sub>x::nat)"
-    by (auto simp add:max_vote_def) (metis (lifting) not_None_eq option.simps(4)) 
-  with max_voted_round_some obtain a where
-    "a |\<in>| q" and "vote r a b\<^sub>m\<^sub>a\<^sub>x \<noteq> None" and 1:"b\<^sub>m\<^sub>a\<^sub>x \<le> bound" by metis
-  hence 
-    "let a2 = SOME a . a |\<in>| q \<and> vote r a b\<^sub>m\<^sub>a\<^sub>x \<noteq> None in a2 |\<in>| q \<and> vote r a2 b\<^sub>m\<^sub>a\<^sub>x \<noteq> None"
-      by (metis (mono_tags, lifting) someI_ex)
-  moreover have "\<And> a2 b2 . \<lbrakk>a2 |\<in>| q; b2 \<le> bound; b2 > b\<^sub>m\<^sub>a\<^sub>x\<rbrakk> \<Longrightarrow> vote r a2 b2 = None" 
-    using max_voted_round_none by (metis "0" option.sel)  
-  moreover have "max_vote r q bound = (vote r) (SOME a . a |\<in>| q \<and> vote r a b\<^sub>m\<^sub>a\<^sub>x \<noteq> None) b\<^sub>m\<^sub>a\<^sub>x"
-    using 0 by (auto simp add:max_vote_def)
-  ultimately show ?thesis using that 1
-    by (metis (no_types, lifting))
-qed
-
-lemma max_vote_none_prop:
-  assumes "max_vote r q (bound::nat) = None"
-  shows "\<And> a b . \<lbrakk>a |\<in>| q; b \<le> bound\<rbrakk> \<Longrightarrow> vote r a b = None"
-using assms
-apply (simp add:max_vote_def split add:option.split_asm)
-    apply (smt max_voted_round_none)
-  apply (smt Paxos.max_voted_round_some Paxos_axioms not_None_eq option.simps(3) someI_ex)
-done
-  
-definition proved_safe_at where
-  "proved_safe_at r Q b v \<equiv>
-    case b of 0 \<Rightarrow> True
-  | Suc c \<Rightarrow> (case (max_vote r Q c) of (* note that here c is b-1 *)
-      None \<Rightarrow> True
-    | Some v' \<Rightarrow> v = v')"
-
-definition chosen_at where
-  "chosen_at r v b \<equiv> \<exists> q . q |\<in>| quorums \<and> (\<forall> a . a |\<in>| q \<longrightarrow> (vote r) a b = (Some v))"
-
-definition chosen where
-  "chosen r v \<equiv> \<exists> b . chosen_at r v b"
-  
-definition choosable where
-  "choosable r v b \<equiv>
-    \<exists> q . q |\<in>| quorums \<and> (\<forall> a . a |\<in>| q \<longrightarrow> (
-      (ballot r a) > Some b \<longrightarrow> (vote r) a b = Some v))"
-
-definition safe_at where
-  "safe_at r v b \<equiv>
-    (\<forall> b2 . \<forall> v2 .
-      ((b2 < b \<and> choosable r v2 b2) \<longrightarrow> (v = v2)))"
-
-definition safe where
-  "safe r \<equiv> \<forall> b . \<forall> a . a |\<in>| acceptors \<longrightarrow> 
-    (let vote = (vote r) a b in (vote \<noteq> None \<longrightarrow> safe_at r (the vote) b))"
-  
-definition well_formed where
-  "well_formed r \<equiv> \<forall> a b . a |\<in>| acceptors \<and> (ballot r) a < b  
-    \<longrightarrow> (vote r) a (the b) = None"
-
-lemma "safe_at r v (bot::nat)"
-by (auto simp add:safe_at_def)
-
-lemma chosen_at_is_choosable:
-  assumes "chosen_at r v b"
-  shows "choosable r v b" using assms
-  by (auto simp add:chosen_at_def choosable_def)
-
-lemma safe_at_prec:
-  assumes "safe_at r v (b::nat)" and "b2 < b"
-  shows "safe_at r v b2"
-  using assms by (meson order.strict_trans safe_at_def)
-
-lemma quorum_inter_witness:
-  assumes "q1 |\<in>| quorums" and "q2 |\<in>| quorums"
-  obtains a where "a |\<in>| q1" and "a |\<in>| q2"
-  using assms Paxos_axioms Paxos_def
-  by (metis all_not_fin_conv finter_iff)
-
-lemma quorum_vote:
-  assumes "q1 |\<in>| quorums" and "q2 |\<in>| quorums"
-  and "\<And> a . a |\<in>| q1 \<Longrightarrow> vote r a b = Some v1"
-  and "\<And> a . a |\<in>| q2 \<Longrightarrow> vote r a b = Some v2"
-  shows "v1 = v2"
-proof -
-  obtain a where "a |\<in>| q1" and "a |\<in>| q2"
-  proof -
-    have "q1 |\<inter>| q2 \<noteq> {||}" using assms(1,2)
-      by (metis Paxos_axioms Paxos_def)
-    hence "\<exists> a . a |\<in>| q1 \<and> a |\<in>| q2"
-      by (metis assms(1) assms(2) quorum_inter_witness) 
-    with that show ?thesis by auto
-  qed
-  thus ?thesis using assms(3,4) by force
-qed
-
-lemma chosen_at_same:
-  assumes "chosen_at r v1 b1" and "chosen_at r v2 b1"
-  shows "v1 = v2" using quorum_vote assms
-  by (auto simp add:chosen_at_def) fast
-
-lemma all_choosable_no_safe:
-  assumes "\<And> (v::'v) . choosable r v b"
-  and "safe_at r v (Suc b)" and "(v1::'v) \<noteq> v2"
-  shows False using assms 
-  by (auto simp add:safe_at_def)(metis lessI)
-
-lemma safe_is_safe:
-  assumes "safe r" and "chosen r v\<^sub>1" and "chosen r v\<^sub>2"
-  shows "v\<^sub>1 = v\<^sub>2"
-  -- {* This follows the proof of Proposition 1 from "Generalized Consensus and Paxos" *}
-proof -
-  text {* The main argument as a lemma to avoid repetitions*}
-  { fix b\<^sub>1 b\<^sub>2 v\<^sub>1 v\<^sub>2
-    assume 1:"chosen_at r v\<^sub>1 b\<^sub>1" and 2:"chosen_at r v\<^sub>2 b\<^sub>2"
-    with this obtain q\<^sub>1 and q\<^sub>2 where 3:"\<And> a . a |\<in>| q\<^sub>1 \<Longrightarrow> (vote r) a b\<^sub>1 = (Some v\<^sub>1)" 
-    and 4:"\<And> a . a |\<in>| q\<^sub>2 \<Longrightarrow> (vote r) a b\<^sub>2 = (Some v\<^sub>2)" and 5:"q\<^sub>1 |\<in>| quorums" and 6:"q\<^sub>2 |\<in>| quorums"
-    by (auto simp add:chosen_at_def)
-    have "v\<^sub>1 = v\<^sub>2" if "b\<^sub>1 < b\<^sub>2"
-    proof -
-      have 9:"choosable r v\<^sub>1 b\<^sub>1" using 1 chosen_at_is_choosable by fast
-      have 10:"safe_at r v\<^sub>2 b\<^sub>2"
-      proof -
-        obtain a where "a |\<in>| q\<^sub>2" using 6 by (metis quorum_inter_witness)
-        with this assms(1) 4 6 have "safe_at r (the (vote r a b\<^sub>2)) b\<^sub>2" 
-          using Paxos_axioms Paxos_def apply auto (* Prood reconstruction fails without calling auto first *)
-            by (metis Paxos_def fset_rev_mp option.discI option.sel safe_def)
-        moreover have "the (vote r a b\<^sub>2) = v\<^sub>2" using `a |\<in>| q\<^sub>2` 4 by force
-        ultimately show ?thesis by auto
-      qed
-      thus ?thesis using 9 10 assms(1) that by (metis safe_at_def)
-    qed }
-  note main = this
-  obtain b\<^sub>1 and b\<^sub>2 where 1:"chosen_at r v\<^sub>1 b\<^sub>1" and 2:"chosen_at r v\<^sub>2 b\<^sub>2" using assms(2,3)
-  by (auto simp add:chosen_def)
-  have ?thesis if "b\<^sub>1 = b\<^sub>2" by (metis "1" "2" chosen_at_same that)
-  moreover
-  have ?thesis if "b\<^sub>1 < b\<^sub>2" using main 1 2 that by blast
-  moreover 
-  have ?thesis if "b\<^sub>2 < b\<^sub>1" using main 1 2 that by blast
-  ultimately show ?thesis by fastforce
-qed
-
-text {* The main lemma *}
-
-lemma proved_safe_is_safe:
-  assumes "safe s" and "q |\<in>| quorums"
-  and "\<And> a . a |\<in>| q \<Longrightarrow> ballot s a \<ge> Some i"
-  and "proved_safe_at s q i v" and "conservative_array s"
-  shows "safe_at s v (i::nat)"
-proof (cases "i = 0")
-  case True thus ?thesis
-    by (metis not_less0 safe_at_def) 
-next
-  case False
-  consider 
-    (a) k a
-      where "a |\<in>| q" and "vote s a k = Some v" and "k < i"
-      and "\<And> a\<^sub>2 l . \<lbrakk>a\<^sub>2 |\<in>| q; k < l; l < i\<rbrakk> \<Longrightarrow> vote s a\<^sub>2 l = None"
-  | (b) "\<And> a k . \<lbrakk>a |\<in>| q; k < i\<rbrakk>  \<Longrightarrow> vote s a k = None"
-  proof (cases "max_vote s q (i-1)")
-    case None 
-    hence "\<And> a k . \<lbrakk>a |\<in>| q; k < i\<rbrakk>  \<Longrightarrow> vote s a k = None" 
-      using False by (metis Suc_diff_eq_diff_pred Suc_leI diff_is_0_eq gr0I max_vote_none_prop)
-    thus ?thesis using that by auto
-  next
-    case (Some v') 
-    with this obtain k a where "a |\<in>| q" and "vote s a k = Some v" and "k < i"  
-      and "\<And> a\<^sub>2 l . \<lbrakk>a\<^sub>2 |\<in>| q; k < l; l < i\<rbrakk> \<Longrightarrow> vote s a\<^sub>2 l = None"
-      using False assms(4)
-      by (simp add:proved_safe_at_def)
-      (smt False Nitpick.case_nat_unfold Some Suc_pred less_Suc_eq_le max_vote_some_prop option.case_eq_if option.sel option.simps(3)) 
-    thus ?thesis using that by auto
-  qed
-  thus ?thesis
-  proof (cases)
-    case b
-    { fix j v
-      assume 1:"j < i"  and 2:"choosable s v j"
-      from 2 obtain q2 where 3:"q2 |\<in>| quorums" and 4:"\<And> a . a |\<in>| q2 \<Longrightarrow>
-        (ballot s a) > Some j \<Longrightarrow> (vote s) a j = Some v"
-        by (auto simp add:choosable_def)
-      from 3 assms(2) obtain a where 5:"a |\<in>| q" and 6:"a |\<in>| q2"
-        using quorum_inter_witness by metis
-      have 9:"vote s a j = Some v"
-        by (metis (no_types, hide_lams) "1" "4" "5" "6" assms(3) less_def less_o.simps(4) not_le order_trans) 
-      from b have False by (metis "1" "5" "9" option.distinct(1)) }
-    thus ?thesis by (auto simp add:safe_at_def)
-  next
-    case a
-    have "v' = v" if "choosable s v' j" and "j < i" for j v'
-    proof -
-      consider (aa) "j < k" | (bb) "j = k" | (cc) "k < j" by fastforce
-      hence ?thesis
-      proof cases
-        case aa
-        have "a |\<in>| acceptors"
-          by (metis Paxos_axioms Paxos_def a(1) assms(2) fset_mp) 
-        hence "safe_at s v k" using  assms(1)
-          by (metis a(2) option.discI option.sel safe_def)
-        with aa show ?thesis using that by (metis safe_at_def) 
-      next
-        case cc
-        from that obtain q2 where 3:"q2 |\<in>| quorums" and 4:"\<And> a . a |\<in>| q2 \<Longrightarrow>
-          (ballot s a) > Some j \<Longrightarrow> (vote s) a j = Some v'"
-          by (auto simp add:choosable_def)
-        from 3 assms(2) obtain a2 where 5:"a2 |\<in>| q" and 6:"a2 |\<in>| q2" 
-          using quorum_inter_witness by metis
-        have 8:"vote s a2 j = Some v'"
-          by (metis (mono_tags, lifting) "4" "5" "6" assms(3) leD leI less_eq_def less_eq_o.simps(3) order_trans that(2)) 
-        show ?thesis using a(4) 5 that(2) 8 cc by (metis option.distinct(1))
-      next
-        case bb (* Here we probably need the fact that the array is conservative: *)
-        have 1:"vote s a k = Some v" if "a |\<in>| acceptors" and " vote s a k \<noteq> None"  for a using that assms(5) 
-          by (auto simp add:conservative_array_def conservative_def)
-            (metis (no_types, hide_lams) Paxos_axioms Paxos_def a(1) a(2) assms(2) option.inject order.not_eq_order_implies_strict pfsubsetD)  
-        from that obtain q2 where 3:"q2 |\<in>| quorums" and 4:"\<And> a . a |\<in>| q2 \<Longrightarrow>
-          (ballot s a) > Some j \<Longrightarrow> (vote s) a j = Some v'"
-          by (auto simp add:choosable_def)
-        from 3 assms(2) obtain a2 where 5:"a2 |\<in>| q" and 6:"a2 |\<in>| q2" 
-          using quorum_inter_witness by metis
-        have 7:"ballot s a2 \<ge> Some k"
-          by (metis "5" a(3) assms(3) less_eq_def less_eq_o.simps(3) less_imp_le order_trans)
-        have 8:"a2 |\<in>| acceptors"
-          by (metis "5" Paxos_axioms Paxos_def assms(2) order.not_eq_order_implies_strict pfsubsetD) 
-        have 9:"vote s a2 k = Some v"
-          by (metis "1" "4" "5" "6" "7" "8" assms(3) bb leD less_eq_def less_eq_o.simps(3) option.discI order.not_eq_order_implies_strict that(2))
-        show ?thesis
-          by (metis "4" "5" "6" "7" "9" antisym_conv2 assms(3) bb leD less_eq_def less_eq_o.simps(3) option.sel that(2)) 
-      qed
-      thus ?thesis by (auto simp add:safe_at_def)
-    qed
-    thus ?thesis
-    by (metis Paxos.safe_at_def Paxos_axioms) 
-  qed 
-qed
-  
-section {* Paxos IOA *}
 
 definition p_asig where
   "p_asig \<equiv>
@@ -369,7 +52,7 @@ definition join_ballot where
 
 definition start_ballot where
   "start_ballot b s s' \<equiv> suggestion s b = None \<and>
-    (\<exists> q v . q |\<in>| quorums \<and> proved_safe_at s q b v \<and> (\<forall> a . a |\<in>| q \<longrightarrow> ballot s a \<ge> Some b)
+    (\<exists> q v . q |\<in>| quorums \<and> ballot_array.proved_safe_at (vote s) q b v \<and> (\<forall> a . a |\<in>| q \<longrightarrow> ballot s a \<ge> Some b)
       \<and> v |\<in>| propCmd s \<and> s' = s\<lparr>suggestion := (suggestion s)(b := Some v)\<rparr>)"
 
 definition do_vote where
@@ -377,7 +60,7 @@ definition do_vote where
     bo \<noteq> None \<and> vote s a b = None \<and> s' = s\<lparr>vote := (vote s)(a := (vote s a)(b := suggestion s b))\<rparr>"
 
 definition learn where
-  "learn l v s s' \<equiv> chosen s v \<and> s = s'"
+  "learn l v s s' \<equiv> ((ballot_array.chosen (vote s) quorums) v) \<and> s = s'"
 
 fun p_trans_fun  where
   "p_trans_fun r (Propose c) r' = propose c r r'"
@@ -392,17 +75,24 @@ definition p_trans where
 definition p_ioa where
   "p_ioa \<equiv> \<lparr>ioa.asig = p_asig, start = p_start, trans = p_trans\<rparr>"
 
-end 
+end
 
 section {* Correctness proof *}
 
 text {* We create a locale for the proof in order to fix the type variables appearing in p_ioa_def
   Otherwise we run into problem with polymorphism and Eisbach *}
 
-locale paxos_proof = IOA + Paxos +
-  fixes the_ioa
+print_locale paxos
+
+locale paxos_proof = IOA + paxos acceptors quorums learners for acceptors :: "'a fset" 
+  and quorums and learners :: "'l fset" +
+  fixes the_ioa :: "(('v,'a)p_state, ('v,'a,'l)p_action) ioa"
   defines "the_ioa \<equiv> p_ioa"
 begin
+
+(* TODO: is this necessary?
+interpretation ba?:ballot_array quorums acceptors "p_state.ballot r" "p_state.vote r" for r::"('v,'a)p_state"
+by (unfold_locales) *)
 
 lemmas p_ioa_defs =  
    is_trans_def actions_def p_trans_def p_start_def
@@ -431,40 +121,44 @@ apply (metis (no_types, lifting) map_upd_Some_unfold option.discI p_state.ext_in
 done
 
 (* Does not seem needed. Is it? *)
-declare well_formed_def[inv_proofs_defs]
+declare ballot_array.well_formed_def[inv_proofs_defs]
 lemma well_formed_inductive:
-  "invariant the_ioa well_formed"
+  "invariant the_ioa (\<lambda> s . ballot_array.well_formed (ballot s) (vote s) acceptors)"
 apply try_solve_inv2
 apply auto
 apply (smt fun_upd_apply gt_not_none neq_iff option.collapse option.sel p_state.ext_inject p_state.surjective p_state.update_convs(3))
-done
-(*declare well_formed_inductive[invs]*)
+done 
+declare well_formed_inductive[invs]
 
-declare conservative_array_def[inv_proofs_defs]
+declare ballot_array.conservative_array_def[inv_proofs_defs]
+abbreviation conservative_array where 
+"conservative_array \<equiv> (\<lambda> s . ballot_array.conservative_array (vote s) acceptors)"
 lemma conservative_inductive:
   "invariant the_ioa conservative_array"
-apply (try_solve_inv2 inv_proofs_defs:inv_proofs_defs conservative_def invs:invs inv1)
-apply metis
-apply metis
+apply (try_solve_inv2 inv_proofs_defs:inv_proofs_defs ballot_array.conservative_def invs:invs inv1)
+    apply metis
+  apply force
 done
 declare conservative_inductive[invs]
 
+abbreviation safe_at where "safe_at \<equiv> \<lambda> s . ballot_array.safe_at (ballot s) (vote s) quorums"
 lemma safe_mono:
   assumes "safe_at s v b" and "s \<midarrow>a\<midarrow>the_ioa\<longrightarrow> t"
   shows "safe_at t v b" using assms
 apply (cases a)
-        apply (auto simp add:inv_proofs_defs safe_at_def choosable_def)[2] (* propose, learn *)
+        apply (auto simp add:inv_proofs_defs ballot_array.safe_at_def ballot_array.choosable_def)[2] (* propose, learn *)
     defer (* join_ballot *)
-    apply (simp add:inv_proofs_defs safe_at_def choosable_def)[1]
+    apply (simp add:inv_proofs_defs ballot_array.safe_at_def ballot_array.choosable_def)[1]
     apply (metis less_def order.strict_trans) 
   defer (* vote *)
-  apply (simp add:inv_proofs_defs safe_at_def choosable_def)
+  apply (simp add:inv_proofs_defs ballot_array.safe_at_def ballot_array.choosable_def)
   apply (smt fun_upd_apply neq_iff option.sel p_state.select_convs(2) p_state.select_convs(3) p_state.surjective p_state.update_convs(3))
   (* That was amazing, Sledgehammer found it before I had time to think about why it would be true... *)
-apply (simp add:inv_proofs_defs safe_at_def choosable_def) (* start_ballot *)
+apply (simp add:inv_proofs_defs ballot_array.safe_at_def ballot_array.choosable_def) (* start_ballot *)
 apply (metis p_state.ext_inject p_state.surjective p_state.update_convs(4))
 done
 
+abbreviation safe where "safe \<equiv> \<lambda> s . ballot_array.safe (ballot s) (vote s) quorums acceptors"
 definition inv2 where
   "inv2 s \<equiv> safe s \<and> (\<forall> b . case suggestion s b of None \<Rightarrow> True | Some v \<Rightarrow> safe_at s v b)"
 declare inv2_def[inv_proofs_defs]
@@ -472,17 +166,17 @@ declare inv2_def[inv_proofs_defs]
 lemma inv2:
   "invariant the_ioa inv2"
 apply(rule invariantI)
-    apply (force simp add:inv_proofs_defs safe_def)
+    apply (force simp add:inv_proofs_defs ballot_array.safe_def)
   apply instantiate_invs_2
   apply (case_tac a)
           subgoal premises prems for s t a v
           proof -
-            from prems(2,5) have 1:"propose v s t"
-              by(auto simp add:inv_proofs_defs) 
+            from prems(2,7) have 1:"propose v s t"
+              by (auto simp add:inv_proofs_defs) 
             hence 2:"\<And> b . suggestion s b = suggestion t b" 
               by(auto simp add:inv_proofs_defs)
             have 3:"safe t" using 1 prems(1) 
-              by (auto simp add:inv_proofs_defs safe_def safe_at_def choosable_def) 
+              by (auto simp add:inv_proofs_defs ballot_array.safe_def ballot_array.safe_at_def ballot_array.choosable_def) 
             from 1 2 3 safe_mono show ?thesis 
               by (auto simp add:inv2_def)
                 (metis inv2_def option.case_eq_if prems(1) prems(2))
@@ -490,65 +184,69 @@ apply(rule invariantI)
         subgoal by (auto simp add:inv_proofs_defs) (* learn *)
       subgoal premises prems for s t act a
       proof - 
-        from prems(2,5) have 1:"do_vote a s t"
+        from prems(2,7) have 1:"do_vote a s t"
           by(auto simp add:inv_proofs_defs)
         hence 2:"\<And> b . suggestion s b = suggestion t b" 
           by (auto simp add:inv_proofs_defs)
             (metis p_state.ext_inject p_state.surjective p_state.update_convs(3))
-        have 3:"safe t" using prems(1) 1 apply(auto simp add:inv2_def safe_def)
-        proof - (* Auto-generated *)
-          fix b :: nat and aa :: 'a
-          assume a1: "let bo = ballot s a; b = the bo in (\<exists>y. bo = Some y) \<and> vote s a b = None \<and> t = s \<lparr>vote := (vote s)(a := (vote s a)(b := suggestion s b))\<rparr>"
-          assume a2: "\<forall>b a. a |\<in>| acceptors \<longrightarrow> (let vote = vote s a b in (\<exists>y. vote = Some y) \<longrightarrow> safe_at s (the vote) b)"
-          assume a3: "\<forall>b. case suggestion s b of None \<Rightarrow> True | Some v \<Rightarrow> safe_at s v b"
-          assume a4: "aa |\<in>| acceptors"
-          { fix cc :: 'c
-            have ff1: "\<forall>p. \<exists>f fa fb fc u. p = \<lparr>propCmd = f::'c fset, ballot = fa::'a \<Rightarrow> nat option, vote = fb, suggestion = fc, \<dots> = u::unit\<rparr>"
-              by (metis p_state.cases_scheme)
-            obtain nn :: nat where
-              ff2: "ballot s a = Some nn \<and> vote s a (the (ballot s a)) = None \<and> t = s \<lparr>vote := (vote s) (a := (vote s a) (the (ballot s a) := suggestion s (the (ballot s a))))\<rparr>"
-              using a1 by metis
-            then have ff3: "vote t = (vote s) (a := (vote s a)(the (Some nn) := suggestion s (the (Some nn))))"
-              using ff1 by (metis p_state.select_convs(3) p_state.update_convs(3))
-            then have ff4: "vote t a = (vote s a)(the (Some nn) := suggestion s (the (Some nn)))"
-              by (metis fun_upd_apply)
-            then have ff5: "vote t a (the (Some nn)) = suggestion s (the (Some nn))"
-              by (metis fun_upd_apply)
-            have ff6: "\<And>aa. vote t aa = vote s aa \<or> a = aa"
-              using ff3 by (metis fun_upd_apply)
-            have "\<And>n. vote t a n = vote s a n \<or> the (Some nn) = n"
-              using ff4 by (metis fun_upd_apply)
-            then have "vote t aa b \<noteq> Some cc \<or> safe_at t (the (vote t aa b)) b"
-              using ff6 ff5 ff2 a4 a3 a2 by (metis option.case_eq_if prems(2) safe_mono) }
-          then show "let z = vote t aa b in (\<exists>c. z = Some c) \<longrightarrow> safe_at t (the z) b"
-            by metis
-        qed
+        have 3:"safe t" using prems(1) 1 apply(auto simp add:inv2_def ballot_array.safe_def)
+          proof - (* Auto-generated by Sledgehammer *)
+            fix b :: nat and aa :: 'a
+            assume a1: "aa |\<in>| acceptors"
+            assume a2: "let bo = ballot s a; b = the bo in (\<exists>y. bo = Some y) \<and> vote s a b = None \<and> t = s \<lparr>vote := (vote s)(a := (vote s a)(b := suggestion s b))\<rparr>"
+            assume a3: "\<forall>b. case suggestion s b of None \<Rightarrow> True | Some v \<Rightarrow> safe_at s v b"
+            assume a4: "\<forall>b a. a |\<in>| acceptors \<longrightarrow> (let vote = vote s a b in (\<exists>y. vote = Some y) \<longrightarrow> safe_at s (the vote) b)"
+            { fix vv :: 'v
+              have ff1: "\<And>n. suggestion s n = None \<or> safe_at s (the (suggestion s n)) n"
+                using a3 by (metis option.case_eq_if)
+              obtain nn :: nat where
+                ff2: "s\<lparr>vote := (vote s) (a := (vote s a) (the (ballot s a) := suggestion s (the (ballot s a))))\<rparr> = t \<and> ballot s a = Some nn \<and> vote s a (the (ballot s a)) = None"
+                using a2 by metis
+              have "\<forall>p. \<exists>f fa fb fc u. \<lparr>propCmd = f::'v fset, ballot = fa::'a \<Rightarrow> nat option, vote = fb, suggestion = fc, \<dots> = u::unit\<rparr> = p"
+                by (metis p_state.cases_scheme)
+              then obtain ff :: "('v, 'a) p_state \<Rightarrow> 'v fset" and zz :: "('v, 'a) p_state \<Rightarrow> 'a \<Rightarrow> nat option" and zza :: "('v, 'a) p_state \<Rightarrow> 'a \<Rightarrow> nat \<Rightarrow> 'v option" and zzb :: "('v, 'a) p_state \<Rightarrow> nat \<Rightarrow> 'v option" and uu :: "('v, 'a) p_state \<Rightarrow> unit" where
+                ff3: "\<And>p. \<lparr>propCmd = ff p, ballot = zz p, vote = zza p, suggestion = zzb p, \<dots> = uu p\<rparr> = p"
+                by moura
+              then have ff4: "\<And>p. vote p = zza p"
+                by (metis p_state.select_convs(3))
+              have "(zza s)(a := (zza s a)(the (Some nn) := suggestion s (the (Some nn)))) = zza t"
+                using ff3 ff2 by (metis p_state.select_convs(3) p_state.update_convs(3))
+              then have "zza t aa b = Some vv \<longrightarrow> ballot_array.safe_at (ballot s) (zza s) quorums (the (Some vv)) b"
+                using ff4 ff2 ff1 a4 a1 by (metis fun_upd_apply)
+              then have "vote t aa b \<noteq> Some vv \<or> safe_at t (the (vote t aa b)) b"
+                using ff4 by (metis prems(2) safe_mono) }
+            then show "let z = vote t aa b in (\<exists>v. z = Some v) \<longrightarrow> safe_at t (the z) b"
+              by metis
+          qed
         from 1 2 3 safe_mono show ?thesis 
           by (auto simp add:inv2_def)
             (metis inv2_def option.case_eq_if prems(1) prems(2))
       qed
     subgoal premises prems for s t act b a
     proof -
-      from prems(2,5) have 1:"join_ballot a b s t"
-        by(auto simp add:inv_proofs_defs)
+      from prems(2,7) have 1:"join_ballot a b s t"
+        by (auto simp add:inv_proofs_defs)
       hence 2:"\<And> b . suggestion s b = suggestion t b" 
         by (auto simp add:inv_proofs_defs)
-      have 3:"safe t" using prems(1) 1 by (auto simp add:inv2_def safe_def) (metis prems(2) safe_mono)
+      have 3:"safe t" using prems(1) 1 apply (auto simp add:inv2_def ballot_array.safe_def)
+        by (metis p_state.ext_inject p_state.surjective p_state.update_convs(2) prems(2) safe_mono) 
       from 1 2 3 safe_mono show ?thesis 
         by (auto simp add:inv2_def)
           (metis inv2_def option.case_eq_if prems(1) prems(2))
     qed
   subgoal premises prems for s t act b
   proof -
-    from prems(2,5) have 1:"start_ballot b s t"
+    from prems(2,7) have 1:"start_ballot b s t"
       by(auto simp add:inv_proofs_defs)
-    have 3:"safe t" using prems(1) 1 by (auto simp add:inv2_def safe_def) (metis prems(2) safe_mono)
-    from 1 obtain q v where 2:"q |\<in>| quorums" and 4:"proved_safe_at s q b v" 
+    have 3:"safe t" using prems(1) 1 by (auto simp add:inv2_def ballot_array.safe_def)
+    from 1 obtain q v where 2:"q |\<in>| quorums" and 4:"(ballot_array.proved_safe_at (vote s)) q b v" 
       and 5:"t = s\<lparr>suggestion := suggestion s(b \<mapsto> v)\<rparr>" and 6:"\<And> a . a |\<in>| q \<Longrightarrow> ballot s a \<ge> Some b"
       by auto
+    interpret ba_props:ballot_array_props "ballot s" "vote s" by unfold_locales
     have 2:"\<And> b . case suggestion t b of None \<Rightarrow> True | Some v \<Rightarrow> safe_at t v b"
-      using 1 2 4 5 6 prems(1,2,3) apply(simp add:inv2_def)
-        by (metis option.case_eq_if proved_safe_is_safe safe_mono)
+      using 1 2 4 5 6 prems(1,2,3)
+        by (simp add:inv2_def)
+          (simp add: ba_props.proved_safe_is_safe option.case_eq_if prems(4))
     from 2 3 show ?thesis by (auto simp add:inv2_def)
   qed
 done
@@ -557,25 +255,26 @@ declare inv2[invs]
 lemma safe_inv:
   "invariant the_ioa safe"
 apply(rule invariantI)
-    apply (force simp add:safe_def inv_proofs_defs)
+    apply (force simp add:ballot_array.safe_def inv_proofs_defs)
   apply instantiate_invs_2
   apply (case_tac a)
-          apply (force simp add:safe_def inv_proofs_defs safe_at_def choosable_def)
-        apply (force simp add:safe_def inv_proofs_defs safe_at_def choosable_def)
+          apply (force simp add:ballot_array.safe_def inv_proofs_defs ballot_array.safe_at_def ballot_array.choosable_def)
+        apply (force simp add:ballot_array.safe_def inv_proofs_defs ballot_array.safe_at_def ballot_array.choosable_def)
       apply (auto simp add:is_trans_def the_ioa_def p_ioa_def p_trans_def inv2_def)
 done
 declare safe_inv[invs]
 
 definition agreement where 
-  "agreement s \<equiv> \<forall> v w . chosen s v \<and> chosen s w \<longrightarrow> v = w"
+  "agreement s \<equiv> \<forall> v w . (ballot_array.chosen (vote s) quorums v) 
+    \<and> ballot_array.chosen (vote s) quorums w \<longrightarrow> v = w"
 lemma agreement:"invariant the_ioa agreement"
 apply(rule invariantI)
-    apply(auto simp add: inv_proofs_defs agreement_def chosen_def chosen_at_def)[1]
+    apply(auto simp add: inv_proofs_defs agreement_def ballot_array.chosen_def ballot_array.chosen_at_def)[1]
     apply (metis fempty_iff quorum_inter_witness)
   apply instantiate_invs_2
-  apply (insert safe_is_safe)
-  apply (force simp add:agreement_def)
-done
+  apply (insert ballot_array_props.safe_is_safe)
+  apply (auto simp add:agreement_def)
+  using ballot_array_props.intro quorums_axioms by fastforce
 
 end
 
