Isabelle2/Quorums.thy
@@ -1,0 +1,29 @@
+theory Quorums
+imports Main 
+  "~~/src/HOL/Library/FSet"
+begin
+
+locale quorums =
+  fixes acceptors::"'a fset" and quorums::"'a fset fset"
+  assumes "acceptors \<noteq> {||}"
+    and "\<And> q1 q2 . \<lbrakk>q1 |\<in>| quorums; q2 |\<in>| quorums\<rbrakk> \<Longrightarrow> q1 |\<inter>| q2 \<noteq> {||}"
+    and "\<And> q . q |\<in>| quorums \<Longrightarrow> q |\<subseteq>| acceptors"
+    and "quorums \<noteq> {||}"
+begin
+
+lemma quorum_inter_witness:
+  assumes "q1 |\<in>| quorums" and "q2 |\<in>| quorums"
+  obtains a where "a |\<in>| q1" and "a |\<in>| q2"
+  using assms quorums_axioms
+    by (meson all_not_fin_conv finter_iff quorums_def)
+
+lemma quorums_value_same:
+  assumes "q1 |\<in>| quorums" and "q2 |\<in>| quorums"
+  and "\<And> a . a |\<in>| q1 \<Longrightarrow> f a = x"
+  and "\<And> a . a |\<in>| q2 \<Longrightarrow> f a = y"
+  shows "x = y" using assms
+by (metis quorum_inter_witness) 
+
+end
+
+end
